examples/Turnstile/Einv5_Proofs.thy
@@ -1,0 +1,271 @@
+theory Einv5_Proofs imports Requirements CommonExtraInv_Proofs 
+begin
+theorem extra1: "VC1 Einv5 s0"
+unfolding VC1_def Einv5_def P2_2_inv_part_used_patterns commonExtraInv_def
+by auto
+
+theorem extra2: "VC2 Einv5 env s0  PdOut'value paid'value opened'value"
+unfolding VC2_def Einv5_def
+ apply(rule impI)
+  apply(rule conjI)
+    using cei2 apply((auto simp add: VC2_def)[1];fastforce)
+  apply(unfold commonExtraInv_def)
+  apply(erule conjE)+
+  apply(erule P2_2_inv_saving)
+   apply(auto split: if_splits)
+  done
+
+theorem extra3: "VC3 Einv5 env s0  PdOut'value paid'value opened'value"
+unfolding VC3_def Einv5_def
+ apply(rule impI)
+  apply(rule conjI)
+    using cei3 apply((auto simp add: VC3_def)[1];fastforce)
+  apply(unfold commonExtraInv_def)
+  apply(erule conjE)+
+  apply(erule P2_2_inv_saving)
+   apply(auto split: if_splits)
+  done
+
+theorem extra4: "VC4 Einv5 env s0  PdOut'value paid'value opened'value"
+unfolding VC4_def Einv5_def
+ apply(rule impI)
+  apply(rule conjI)
+    using cei4 apply((auto simp add: VC4_def)[1];fastforce)
+  apply(unfold commonExtraInv_def)
+  apply(erule conjE)+
+  apply(erule P2_2_inv_saving)
+   apply(auto split: if_splits)
+  done
+
+theorem extra5: "VC5 Einv5 env s0  PdOut'value paid'value opened'value"
+unfolding VC5_def Einv5_def
+ apply(rule impI)
+  apply(rule conjI)
+    using cei5 apply((auto simp add: VC5_def)[1];fastforce)
+  apply(unfold commonExtraInv_def)
+  apply(erule conjE)+
+  apply(erule P2_2_inv_saving)
+   apply(auto split: if_splits)
+  done
+
+theorem extra6: "VC6 Einv5 env s0  PdOut'value paid'value opened'value"
+unfolding VC6_def Einv5_def
+ apply(rule impI)
+  apply(rule conjI)
+    using cei6 apply((auto simp add: VC6_def)[1];fastforce)
+  apply(unfold commonExtraInv_def)
+  apply(erule conjE)+
+  apply(erule P2_2_inv_saving)
+   apply(auto split: if_splits)
+  done
+
+theorem extra7: "VC7 Einv5 env s0  PdOut'value paid'value opened'value"
+unfolding VC7_def Einv5_def
+ apply(rule impI)
+  apply(rule conjI)
+    using cei7 apply((auto simp add: VC7_def)[1];fastforce)
+  apply(unfold commonExtraInv_def)
+  apply(erule conjE)+
+  apply(erule P2_2_inv_saving)
+   apply(auto split: if_splits)
+  done
+
+theorem extra8: "VC8 Einv5 env s0  PdOut'value paid'value opened'value"
+unfolding VC8_def Einv5_def
+ apply(rule impI)
+  apply(rule conjI)
+    using cei8 apply((auto simp add: VC8_def)[1];fastforce)
+  apply(unfold commonExtraInv_def)
+  apply(erule conjE)+
+  apply(erule P2_2_inv_saving)
+   apply(auto split: if_splits)
+  done
+
+theorem extra9: "VC9 Einv5 env s0  PdOut'value paid'value opened'value"
+unfolding VC9_def Einv5_def
+ apply(rule impI)
+  apply(rule conjI)
+    using cei9 apply((auto simp add: VC9_def)[1];fastforce)
+  apply(unfold commonExtraInv_def)
+  apply(erule conjE)+
+  apply(erule P2_2_inv_saving)
+   apply(auto split: if_splits)
+  done
+
+theorem extra10: "VC10 Einv5 env s0  PdOut'value paid'value opened'value"
+unfolding VC10_def Einv5_def
+ apply(rule impI)
+  apply(rule conjI)
+    using cei10 apply((auto simp add: VC10_def)[1];fastforce)
+  apply(unfold commonExtraInv_def)
+  apply(erule conjE)+
+  apply(erule P2_2_inv_saving)
+   apply(auto split: if_splits)
+  done
+
+theorem extra11: "VC11 Einv5 env s0  PdOut'value paid'value opened'value"
+unfolding VC11_def Einv5_def
+ apply(rule impI)
+  apply(rule conjI)
+    using cei11 apply((auto simp add: VC11_def)[1];fastforce)
+  apply(unfold commonExtraInv_def)
+  apply(erule conjE)+
+  apply(erule P2_2_inv_saving)
+   apply(auto split: if_splits)
+  done
+
+theorem extra12: "VC12 Einv5 env s0  PdOut'value paid'value opened'value"
+unfolding VC12_def Einv5_def
+ apply(rule impI)
+  apply(rule conjI)
+    using cei12 apply((auto simp add: VC12_def)[1];fastforce)
+  apply(unfold commonExtraInv_def)
+  apply(erule conjE)+
+  apply(erule P2_2_inv_saving)
+   apply(auto split: if_splits)
+  done
+
+theorem extra13: "VC13 Einv5 env s0  PdOut'value paid'value opened'value"
+unfolding VC13_def Einv5_def
+ apply(rule impI)
+  apply(rule conjI)
+    using cei13 apply((auto simp add: VC13_def)[1];fastforce)
+  apply(unfold commonExtraInv_def)
+  apply(erule conjE)+
+  apply(erule P2_2_inv_saving)
+   apply(auto split: if_splits)
+  done
+
+theorem extra14: "VC14 Einv5 env s0  PdOut'value paid'value opened'value"
+unfolding VC14_def Einv5_def
+ apply(rule impI)
+  apply(rule conjI)
+    using cei14 apply((auto simp add: VC14_def)[1];fastforce)
+  apply(unfold commonExtraInv_def)
+  apply(erule conjE)+
+  apply(erule P2_2_inv_saving)
+   apply(auto split: if_splits)
+  done
+
+theorem extra15: "VC15 Einv5 env s0  PdOut'value paid'value opened'value"
+unfolding VC15_def Einv5_def
+ apply(rule impI)
+  apply(rule conjI)
+    using cei15 apply((auto simp add: VC15_def)[1];fastforce)
+  apply(unfold commonExtraInv_def)
+  apply(erule conjE)+
+  apply(erule P2_2_inv_saving)
+   apply(auto split: if_splits)
+  done
+
+theorem extra16: "VC16 Einv5 env s0  PdOut'value paid'value opened'value"
+unfolding VC16_def Einv5_def
+ apply(rule impI)
+  apply(rule conjI)
+    using cei16 apply((auto simp add: VC16_def)[1];fastforce)
+  apply(unfold commonExtraInv_def)
+  apply(erule conjE)+
+  apply(erule P2_2_inv_saving)
+   apply(auto split: if_splits)
+  done
+
+theorem extra17: "VC17 Einv5 env s0  PdOut'value paid'value opened'value"
+unfolding VC17_def Einv5_def
+ apply(rule impI)
+  apply(rule conjI)
+    using cei17 apply((auto simp add: VC17_def)[1];fastforce)
+  apply(unfold commonExtraInv_def)
+  apply(erule conjE)+
+  apply(erule P2_2_inv_saving)
+   apply(auto split: if_splits)
+  done
+
+theorem extra18: "VC18 Einv5 env s0  PdOut'value paid'value opened'value"
+unfolding VC18_def Einv5_def
+ apply(rule impI)
+  apply(rule conjI)
+    using cei18 apply((auto simp add: VC18_def)[1];fastforce)
+  apply(unfold commonExtraInv_def)
+  apply(erule conjE)+
+  apply(erule P2_2_inv_saving)
+   apply(auto split: if_splits)
+  done
+
+theorem extra19: "VC19 Einv5 env s0  PdOut'value paid'value opened'value"
+unfolding VC19_def Einv5_def
+ apply(rule impI)
+  apply(rule conjI)
+    using cei19 apply((auto simp add: VC19_def)[1];fastforce)
+  apply(unfold commonExtraInv_def)
+  apply(erule conjE)+
+  apply(erule P2_2_inv_saving)
+   apply(auto split: if_splits)
+  done
+
+theorem extra20: "VC20 Einv5 env s0  PdOut'value paid'value opened'value"
+unfolding VC20_def Einv5_def
+ apply(rule impI)
+  apply(rule conjI)
+    using cei20 apply((auto simp add: VC20_def)[1];fastforce)
+  apply(unfold commonExtraInv_def)
+  apply(erule conjE)+
+  apply(erule P2_2_inv_saving)
+   apply(auto split: if_splits)
+  done
+
+theorem extra21: "VC21 Einv5 env s0  PdOut'value paid'value opened'value"
+unfolding VC21_def Einv5_def
+ apply(rule impI)
+  apply(rule conjI)
+    using cei21 apply((auto simp add: VC21_def)[1];fastforce)
+  apply(unfold commonExtraInv_def)
+  apply(erule conjE)+
+  apply(erule P2_2_inv_saving)
+   apply(auto split: if_splits)
+  done
+
+theorem extra22: "VC22 Einv5 env s0  PdOut'value paid'value opened'value"
+unfolding VC22_def Einv5_def
+ apply(rule impI)
+  apply(rule conjI)
+    using cei22 apply((auto simp add: VC22_def)[1];fastforce)
+  apply(unfold commonExtraInv_def)
+  apply(erule conjE)+
+  apply(erule P2_2_inv_saving)
+   apply(auto split: if_splits)
+  done
+
+theorem extra23: "VC23 Einv5 env s0  PdOut'value paid'value opened'value"
+unfolding VC23_def Einv5_def
+ apply(rule impI)
+  apply(rule conjI)
+    using cei23 apply((auto simp add: VC23_def)[1];fastforce)
+  apply(unfold commonExtraInv_def)
+  apply(erule conjE)+
+  apply(erule P2_2_inv_saving)
+   apply(auto split: if_splits)
+  done
+
+theorem extra24: "VC24 Einv5 env s0  PdOut'value paid'value opened'value"
+unfolding VC24_def Einv5_def
+ apply(rule impI)
+  apply(rule conjI)
+    using cei24 apply((auto simp add: VC24_def)[1];fastforce)
+  apply(unfold commonExtraInv_def)
+  apply(erule conjE)+
+  apply(erule P2_2_inv_saving)
+   apply(auto split: if_splits)
+  done
+
+theorem extra25: "VC25 Einv5 env s0  PdOut'value paid'value opened'value"
+unfolding VC25_def Einv5_def
+ apply(rule impI)
+  apply(rule conjI)
+    using cei25 apply((auto simp add: VC25_def)[1];fastforce)
+  apply(unfold commonExtraInv_def)
+  apply(erule conjE)+
+  apply(erule P2_2_inv_saving)
+   apply(auto split: if_splits)
+  done
+
+end
