examples/Turnstile/R2_Proofs.thy
@@ -1,0 +1,273 @@
+theory R2_Proofs imports Einv2_Proofs 
+begin
+definition R2_extended_inv where "R2_extended_inv s \<equiv> Einv2 s \<and> R2 s"
+
+theorem extra1: "VC1 R2_extended_inv s0"
+unfolding VC1_def R2_extended_inv_def Einv2_def R2_def always2_inv_part_used_patterns always2_part_used_patterns commonExtraInv_def
+by auto
+
+theorem extendedInv2: "VC2 R2_extended_inv env s0  PdOut'value paid'value opened'value"
+unfolding VC2_def R2_extended_inv_def R2_def  apply(rule impI)
+  apply(rule context_conjI)
+  using extra2 apply((auto simp add: VC2_def)[1];fastforce)
+  apply(rule conjI)
+   apply simp
+  apply(unfold Einv2_def commonExtraInv_def)
+  apply(erule conjE)+
+  apply(auto simp add: always2einv_imp_req)
+  done
+
+theorem extendedInv3: "VC3 R2_extended_inv env s0  PdOut'value paid'value opened'value"
+unfolding VC3_def R2_extended_inv_def R2_def  apply(rule impI)
+  apply(rule context_conjI)
+  using extra3 apply((auto simp add: VC3_def)[1];fastforce)
+  apply(rule conjI)
+   apply simp
+  apply(unfold Einv2_def commonExtraInv_def)
+  apply(erule conjE)+
+  apply(auto simp add: always2einv_imp_req)
+  done
+
+theorem extendedInv4: "VC4 R2_extended_inv env s0  PdOut'value paid'value opened'value"
+unfolding VC4_def R2_extended_inv_def R2_def  apply(rule impI)
+  apply(rule context_conjI)
+  using extra4 apply((auto simp add: VC4_def)[1];fastforce)
+  apply(rule conjI)
+   apply simp
+  apply(unfold Einv2_def commonExtraInv_def)
+  apply(erule conjE)+
+  apply(auto simp add: always2einv_imp_req)
+  done
+
+theorem extendedInv5: "VC5 R2_extended_inv env s0  PdOut'value paid'value opened'value"
+unfolding VC5_def R2_extended_inv_def R2_def  apply(rule impI)
+  apply(rule context_conjI)
+  using extra5 apply((auto simp add: VC5_def)[1];fastforce)
+  apply(rule conjI)
+   apply simp
+  apply(unfold Einv2_def commonExtraInv_def)
+  apply(erule conjE)+
+  apply(auto simp add: always2einv_imp_req)
+  done
+
+theorem extendedInv6: "VC6 R2_extended_inv env s0  PdOut'value paid'value opened'value"
+unfolding VC6_def R2_extended_inv_def R2_def  apply(rule impI)
+  apply(rule context_conjI)
+  using extra6 apply((auto simp add: VC6_def)[1];fastforce)
+  apply(rule conjI)
+   apply simp
+  apply(unfold Einv2_def commonExtraInv_def)
+  apply(erule conjE)+
+  apply(auto simp add: always2einv_imp_req)
+  done
+
+theorem extendedInv7: "VC7 R2_extended_inv env s0  PdOut'value paid'value opened'value"
+unfolding VC7_def R2_extended_inv_def R2_def  apply(rule impI)
+  apply(rule context_conjI)
+  using extra7 apply((auto simp add: VC7_def)[1];fastforce)
+  apply(rule conjI)
+   apply simp
+  apply(unfold Einv2_def commonExtraInv_def)
+  apply(erule conjE)+
+  apply(auto simp add: always2einv_imp_req)
+  done
+
+theorem extendedInv8: "VC8 R2_extended_inv env s0  PdOut'value paid'value opened'value"
+unfolding VC8_def R2_extended_inv_def R2_def  apply(rule impI)
+  apply(rule context_conjI)
+  using extra8 apply((auto simp add: VC8_def)[1];fastforce)
+  apply(rule conjI)
+   apply simp
+  apply(unfold Einv2_def commonExtraInv_def)
+  apply(erule conjE)+
+  apply(auto simp add: always2einv_imp_req)
+  done
+
+theorem extendedInv9: "VC9 R2_extended_inv env s0  PdOut'value paid'value opened'value"
+unfolding VC9_def R2_extended_inv_def R2_def  apply(rule impI)
+  apply(rule context_conjI)
+  using extra9 apply((auto simp add: VC9_def)[1];fastforce)
+  apply(rule conjI)
+   apply simp
+  apply(unfold Einv2_def commonExtraInv_def)
+  apply(erule conjE)+
+  apply(auto simp add: always2einv_imp_req)
+  done
+
+theorem extendedInv10: "VC10 R2_extended_inv env s0  PdOut'value paid'value opened'value"
+unfolding VC10_def R2_extended_inv_def R2_def  apply(rule impI)
+  apply(rule context_conjI)
+  using extra10 apply((auto simp add: VC10_def)[1];fastforce)
+  apply(rule conjI)
+   apply simp
+  apply(unfold Einv2_def commonExtraInv_def)
+  apply(erule conjE)+
+  apply(auto simp add: always2einv_imp_req)
+  done
+
+theorem extendedInv11: "VC11 R2_extended_inv env s0  PdOut'value paid'value opened'value"
+unfolding VC11_def R2_extended_inv_def R2_def  apply(rule impI)
+  apply(rule context_conjI)
+  using extra11 apply((auto simp add: VC11_def)[1];fastforce)
+  apply(rule conjI)
+   apply simp
+  apply(unfold Einv2_def commonExtraInv_def)
+  apply(erule conjE)+
+  apply(auto simp add: always2einv_imp_req)
+  done
+
+theorem extendedInv12: "VC12 R2_extended_inv env s0  PdOut'value paid'value opened'value"
+unfolding VC12_def R2_extended_inv_def R2_def  apply(rule impI)
+  apply(rule context_conjI)
+  using extra12 apply((auto simp add: VC12_def)[1];fastforce)
+  apply(rule conjI)
+   apply simp
+  apply(unfold Einv2_def commonExtraInv_def)
+  apply(erule conjE)+
+  apply(auto simp add: always2einv_imp_req)
+  done
+
+theorem extendedInv13: "VC13 R2_extended_inv env s0  PdOut'value paid'value opened'value"
+unfolding VC13_def R2_extended_inv_def R2_def  apply(rule impI)
+  apply(rule context_conjI)
+  using extra13 apply((auto simp add: VC13_def)[1];fastforce)
+  apply(rule conjI)
+   apply simp
+  apply(unfold Einv2_def commonExtraInv_def)
+  apply(erule conjE)+
+  apply(auto simp add: always2einv_imp_req)
+  done
+
+theorem extendedInv14: "VC14 R2_extended_inv env s0  PdOut'value paid'value opened'value"
+unfolding VC14_def R2_extended_inv_def R2_def  apply(rule impI)
+  apply(rule context_conjI)
+  using extra14 apply((auto simp add: VC14_def)[1];fastforce)
+  apply(rule conjI)
+   apply simp
+  apply(unfold Einv2_def commonExtraInv_def)
+  apply(erule conjE)+
+  apply(auto simp add: always2einv_imp_req)
+  done
+
+theorem extendedInv15: "VC15 R2_extended_inv env s0  PdOut'value paid'value opened'value"
+unfolding VC15_def R2_extended_inv_def R2_def  apply(rule impI)
+  apply(rule context_conjI)
+  using extra15 apply((auto simp add: VC15_def)[1];fastforce)
+  apply(rule conjI)
+   apply simp
+  apply(unfold Einv2_def commonExtraInv_def)
+  apply(erule conjE)+
+  apply(auto simp add: always2einv_imp_req)
+  done
+
+theorem extendedInv16: "VC16 R2_extended_inv env s0  PdOut'value paid'value opened'value"
+unfolding VC16_def R2_extended_inv_def R2_def  apply(rule impI)
+  apply(rule context_conjI)
+  using extra16 apply((auto simp add: VC16_def)[1];fastforce)
+  apply(rule conjI)
+   apply simp
+  apply(unfold Einv2_def commonExtraInv_def)
+  apply(erule conjE)+
+  apply(auto simp add: always2einv_imp_req)
+  done
+
+theorem extendedInv17: "VC17 R2_extended_inv env s0  PdOut'value paid'value opened'value"
+unfolding VC17_def R2_extended_inv_def R2_def  apply(rule impI)
+  apply(rule context_conjI)
+  using extra17 apply((auto simp add: VC17_def)[1];fastforce)
+  apply(rule conjI)
+   apply simp
+  apply(unfold Einv2_def commonExtraInv_def)
+  apply(erule conjE)+
+  apply(auto simp add: always2einv_imp_req)
+  done
+
+theorem extendedInv18: "VC18 R2_extended_inv env s0  PdOut'value paid'value opened'value"
+unfolding VC18_def R2_extended_inv_def R2_def  apply(rule impI)
+  apply(rule context_conjI)
+  using extra18 apply((auto simp add: VC18_def)[1];fastforce)
+  apply(rule conjI)
+   apply simp
+  apply(unfold Einv2_def commonExtraInv_def)
+  apply(erule conjE)+
+  apply(auto simp add: always2einv_imp_req)
+  done
+
+theorem extendedInv19: "VC19 R2_extended_inv env s0  PdOut'value paid'value opened'value"
+unfolding VC19_def R2_extended_inv_def R2_def  apply(rule impI)
+  apply(rule context_conjI)
+  using extra19 apply((auto simp add: VC19_def)[1];fastforce)
+  apply(rule conjI)
+   apply simp
+  apply(unfold Einv2_def commonExtraInv_def)
+  apply(erule conjE)+
+  apply(auto simp add: always2einv_imp_req)
+  done
+
+theorem extendedInv20: "VC20 R2_extended_inv env s0  PdOut'value paid'value opened'value"
+unfolding VC20_def R2_extended_inv_def R2_def  apply(rule impI)
+  apply(rule context_conjI)
+  using extra20 apply((auto simp add: VC20_def)[1];fastforce)
+  apply(rule conjI)
+   apply simp
+  apply(unfold Einv2_def commonExtraInv_def)
+  apply(erule conjE)+
+  apply(auto simp add: always2einv_imp_req)
+  done
+
+theorem extendedInv21: "VC21 R2_extended_inv env s0  PdOut'value paid'value opened'value"
+unfolding VC21_def R2_extended_inv_def R2_def  apply(rule impI)
+  apply(rule context_conjI)
+  using extra21 apply((auto simp add: VC21_def)[1];fastforce)
+  apply(rule conjI)
+   apply simp
+  apply(unfold Einv2_def commonExtraInv_def)
+  apply(erule conjE)+
+  apply(auto simp add: always2einv_imp_req)
+  done
+
+theorem extendedInv22: "VC22 R2_extended_inv env s0  PdOut'value paid'value opened'value"
+unfolding VC22_def R2_extended_inv_def R2_def  apply(rule impI)
+  apply(rule context_conjI)
+  using extra22 apply((auto simp add: VC22_def)[1];fastforce)
+  apply(rule conjI)
+   apply simp
+  apply(unfold Einv2_def commonExtraInv_def)
+  apply(erule conjE)+
+  apply(auto simp add: always2einv_imp_req)
+  done
+
+theorem extendedInv23: "VC23 R2_extended_inv env s0  PdOut'value paid'value opened'value"
+unfolding VC23_def R2_extended_inv_def R2_def  apply(rule impI)
+  apply(rule context_conjI)
+  using extra23 apply((auto simp add: VC23_def)[1];fastforce)
+  apply(rule conjI)
+   apply simp
+  apply(unfold Einv2_def commonExtraInv_def)
+  apply(erule conjE)+
+  apply(auto simp add: always2einv_imp_req)
+  done
+
+theorem extendedInv24: "VC24 R2_extended_inv env s0  PdOut'value paid'value opened'value"
+unfolding VC24_def R2_extended_inv_def R2_def  apply(rule impI)
+  apply(rule context_conjI)
+  using extra24 apply((auto simp add: VC24_def)[1];fastforce)
+  apply(rule conjI)
+   apply simp
+  apply(unfold Einv2_def commonExtraInv_def)
+  apply(erule conjE)+
+  apply(auto simp add: always2einv_imp_req)
+  done
+
+theorem extendedInv25: "VC25 R2_extended_inv env s0  PdOut'value paid'value opened'value"
+unfolding VC25_def R2_extended_inv_def R2_def  apply(rule impI)
+  apply(rule context_conjI)
+  using extra25 apply((auto simp add: VC25_def)[1];fastforce)
+  apply(rule conjI)
+   apply simp
+  apply(unfold Einv2_def commonExtraInv_def)
+  apply(erule conjE)+
+  apply(auto simp add: always2einv_imp_req)
+  done
+
+end
